tapl/coq/03_arith/TSet.v
@@ -1,11 +1,55 @@
-Require Import TAPL_03_Arith.Arith.
-Require Import ListSet.
+Require Import TAPL_03_Arith.Term.
+Require Import TAPL_03_Arith.SetUtil.
+Require Import MSets MSetWeakList.
 
 Theorem Term_eq_dec: forall t1 t2: Term, {t1 = t2} + {t1 <> t2}.
 Proof. decide equality. Defined.
-Definition tset := set Term.
-Definition tset_empty := empty_set Term.
-Definition tset_add := set_add Term_eq_dec.
-Definition tset_single (t: Term) := tset_add t tset_empty.
-Definition tset_union := set_union Term_eq_dec.
-Definition tset_union3 (s1 s2 s3: tset) := tset_union s1 (tset_union s2 s3).
+
+Module DecidableTerm <: UsualDecidableType.
+  Definition t := Term.
+  Definition eq := @eq t.
+  Definition eq_equiv : Equivalence eq := eq_equivalence.
+  Definition eq_dec := Term_eq_dec.
+End DecidableTerm.
+
+Module TSet := Make DecidableTerm.
+Module TSetFacts := Facts TSet.
+Module TSetNotations := SetNotations DecidableTerm TSet.
+Module TSet1 := Set1 DecidableTerm TSet.
+Module TSet2 := Set2 DecidableTerm DecidableTerm TSet TSet.
+
+Section TSetExample.
+  Import TSet.
+  Import TSetNotations.
+
+  Compute singleton TTrue.
+  Check add TFalse (singleton TTrue).
+  Check {TTrue;TZero}.
+  Check TFalse +: {TTrue;TZero}.
+  Check union {TFalse} {TTrue;TZero}.
+
+  Import TSet2.
+  Check map TSucc {TZero; TSucc TZero}.
+End TSetExample.
+
+(* Definition tset := set Term. *)
+(* Definition tset_empty := empty_set Term. *)
+(* Definition tset_add := set_add Term_eq_dec. *)
+(* Definition tset_single (t: Term) := tset_add t tset_empty. *)
+(* Definition tset_union := set_union Term_eq_dec. *)
+(* Definition tset_union3 (s1 s2 s3: tset) := tset_union s1 (tset_union s2 s3). *)
+(* Definition tset_In := set_In (A := Term). *)
+
+(* Fixpoint tset_from_list (ts: list Term) := *)
+(*   match ts with *)
+(*   | nil => tset_empty *)
+(*   | t :: ts' => tset_add t (tset_from_list ts') *)
+(*   end. *)
+
+(* Definition tset_map {A: Type}: (A -> Term) -> set A -> tset := set_map Term_eq_dec. *)
+
+(* Fixpoint tset_flat_map (f: Term -> tset) (ts: tset): tset := *)
+(*   match ts with *)
+(*   | [] => tset_empty *)
+(*   | t :: ts' => tset_union (f t) (tset_flat_map f ts') *)
+(*   end. *)
