tapl/coq/03_arith/LSet.v
@@ -1,0 +1,59 @@
+(** ListSet as a paramtric module *)
+Require Import Arith.
+Require Import ListSet.
+Require List.
+
+Module Type Key.
+  Parameter A: Set.
+  Parameter eq_dec: forall x y:A, {x = y} + {x <> y}.
+End Key.
+
+Module NatKey <: Key.
+  Definition A := nat.
+  Definition eq_dec := Nat.eq_dec.
+End NatKey.
+
+Module LSet(K: Key).
+  Definition set := ListSet.set K.A.
+  Definition empty := empty_set K.A.
+  Definition add := set_add K.eq_dec.
+  Definition single (x: K.A) := add x empty.
+  Definition union := set_union K.eq_dec.
+  Definition union3 (s1 s2 s3: set) := union s1 (union s2 s3).
+  Definition In := @set_In K.A. 
+
+  Declare Scope set_scope.
+  Delimit Scope set_scope with set.
+  Bind Scope set_scope with set.
+
+  Infix "+:" := add (at level 60, right associativity): set_scope.
+  (* Notation "x +: xs" := (add x xs) (at level 60, right associativity). *)
+  Notation "{ }" := empty (format "{ }"): set_scope.
+  Notation "{ x }" := (add x empty) (format "{ x }"): set_scope.
+  Notation "{ x ; .. ; y }" := (add x .. (add y empty) ..)
+                                 (format "{ x ; .. ; y }"): set_scope.
+  Open Scope set_scope.
+
+  Definition map {X: Type}: (X -> K.A) -> ListSet.set X -> set := set_map K.eq_dec.
+
+  Fixpoint flat_map (f: K.A -> set) (s: set): set :=
+    match s with
+    | List.nil => empty
+    | List.cons h t => union (f h) (flat_map f t)
+    end.
+End LSet.
+
+Module NatSet := LSet NatKey.
+
+Section NatSetExample.
+  Import NatSet.
+  Check empty : set. (* {} : set *)
+  Check (add 1 empty) : set. (* {1} : set *)
+  Check 4 +: {} : set. (* {4} : set *)
+  Check {1;2;3} : set. (* {1;2;3} : set *)
+  Check 1 +: 2 +: 3 +: empty : set. (* {1;2;3} : set *)
+  Check map S {1;2;3}. (* map S {1;2;3} : set *)
+  (* Example map_ex: map S {1;2;3} = {2;3;4}. *)
+  (* Proof. simpl. reflexivity. Qed. *)
+
+End NatSetExample.
