tapl/coq/03_arith/MSetEx.v
@@ -1,0 +1,51 @@
+Require Import MSets.
+Require Import MSetList.
+
+Print OrderedTypeWithLeibniz.
+
+Module OWL.
+  Definition t := nat.
+  Definition eq := @eq t.
+  Instance eq_equiv : Equivalence eq := eq_equivalence.
+  Definition lt := lt.
+  Instance lt_strorder : StrictOrder lt := Nat_as_OT.lt_strorder.
+  Instance lt_compat : Proper (eq ==> eq ==> iff) lt.
+  Proof.
+    now unfold eq; split; subst.
+  Qed.
+  SearchPattern (nat -> nat -> comparison).
+  Definition compare := Nat_as_OT.compare.
+  About CompSpec.
+  (*So, nothing here on nat*)
+  Lemma compare_spec : forall x y, CompSpec eq lt x y (compare x y).
+  Proof.
+    (* SearchPattern (forall x y, Compare_dec.nat_compare x y = _ -> _). *)
+    intros; case_eq (compare x y); constructor.
+    now apply Compare_dec.nat_compare_eq.
+    now apply Compare_dec.nat_compare_Lt_lt.
+    now apply Compare_dec.nat_compare_Gt_gt.
+  Qed.
+  SearchPattern (forall (a b:nat), {a=b}+{a<>b}).
+  Definition eq_dec := Peano_dec.eq_nat_dec.
+  Definition eq_leibniz a b (H:eq a b) := H.
+End OWL.
+
+Module NatSet := MakeWithLeibniz OWL.
+
+Inductive exemple :=
+| A : exemple
+| B : NatSet.t -> exemple
+| C : NatSet.t -> bool -> exemple.
+
+Definition eq_dec : forall (a b:exemple), {a=b}+{a<>b}.
+  intros; decide equality.
+  destruct (NatSet.eq_dec t t0).
+  now left; apply NatSet.eq_leibniz.
+  right; intro; apply n; clear n; subst.
+  reflexivity.
+  apply bool_dec.
+  destruct (NatSet.eq_dec t t0).
+  now left; apply NatSet.eq_leibniz.
+  right; intro; apply n; clear n; subst.
+  reflexivity.
+Defined.
