tapl/coq/03_arith/SetUtil.v
@@ -1,0 +1,119 @@
+Require Import MSets MSetWeakList.
+Require Import Setoid.
+
+Module SetNotations (X: DecidableType) (XS: WSetsOn X).
+  Import XS.
+  Declare Scope set_scope.
+  Delimit Scope set_scope with t.
+  Bind Scope set_scope with t.
+
+  Infix "+:" := add (at level 60, right associativity): set_scope.
+  (* Notation "x +: xs" := (add x xs) (at level 60, right associativity). *)
+  Notation "{ }" := empty (format "{ }"): set_scope.
+  Notation "{ x }" := (add x empty) (format "{ x }"): set_scope.
+  Notation "{ x ; .. ; y }" := (add x .. (add y empty) ..)
+                                 (format "{ x ; .. ; y }"): set_scope.
+  Infix "++" := union (right associativity, at level 60) : set_scope.
+  Open Scope set_scope.
+End SetNotations.
+
+(** * defs adn facts about set types *)
+Module Set1 (X: DecidableType) (XS: WSetsOn X).
+  Include XS <+ (WPropertiesOn X XS).
+  (* Import XS. *)
+  (* Module SetProps := WPropertiesOn X XS. *)
+  (* Import SetProps. *)
+  (* Export SetProps. *)
+
+  Definition disjoint (s1 s2: XS.t): Prop :=
+    forall x: X.t, (In x s1 -> ~In x s2) /\ (In x s2 -> ~In x s1).
+
+  Theorem disjoint_iff_inter_is_empty (s1 s2: XS.t):
+    disjoint s1 s2 <-> inter s1 s2 [=] empty.
+  Proof.
+    unfold disjoint. split; intro H; intro x.
+    - destruct (H x) as [H1 H2].
+      split; intro G.
+      + apply inter_spec in G as [G1 G2].
+        apply H1 in G1. contradiction.
+      + rewrite FM.empty_iff in G. contradict G.
+    - pose (H x) as Hx. rewrite inter_spec in Hx.
+      rewrite FM.empty_iff in Hx. rewrite <- neg_false in Hx.
+      split; intros G C; apply Hx; split; assumption.
+  Qed.
+
+  Theorem cardinal_of_disjoint_union (xs ys: XS.t): disjoint xs ys ->
+    cardinal (union xs ys) = cardinal xs + cardinal ys.
+  Proof.
+    intro HD. rewrite disjoint_iff_inter_is_empty in HD.
+    rewrite <- union_inter_cardinal, HD, empty_cardinal.
+    apply plus_n_O.
+  Qed.
+  
+  Theorem fold_add' {A: Type} (f: X.t -> A -> A) (x: X.t) (xs xxs: XS.t) (z: A):
+    ~In x xs -> Add x xs xxs -> fold f xxs z = f x (fold f xs z).
+  Proof.
+    intros Nin Hadd. apply Add_Equal in Hadd. repeat rewrite fold_spec_right.
+    apply fold_add.
+End Set1.
+
+(** * functions on sets and facts about two set types *)
+Module Set2 (X Y: DecidableType) (XS: WSetsOn X) (YS: WSetsOn Y).
+  Module SetXS := Set1 X XS.
+  Module SetYS := Set1 Y YS.
+  
+  Definition map (f: X.t -> Y.t) (xs: XS.t): YS.t :=
+    XS.fold (fun x acc => YS.add (f x) acc) xs YS.empty.
+
+  Definition flat_map (f: X.t -> YS.t) (xs: XS.t): YS.t :=
+    XS.fold (fun x acc => YS.union (f x) acc) xs YS.empty.
+
+  Theorem flat_map_of_empty (f: X.t -> YS.t) (xs: XS.t): XS.Empty xs -> flat_map f xs = YS.empty.
+  Proof.
+    intros Exs. unfold flat_map. rewrite SetXS.fold_1b; try assumption.
+    reflexivity.
+  Qed.
+
+  Definition disjoint_map (f: X.t -> YS.t) (xs: XS.t) :=
+    forall x1 x2: X.t, XS.In x1 xs -> XS.In x2 xs -> x1 <> x2 -> SetYS.disjoint (f x1) (f x2).
+
+  Theorem cardinal_of_disjoint_flat_map (f: X.t -> YS.t) (xs: XS.t):
+    disjoint_map f xs ->
+    YS.cardinal (flat_map f xs) = XS.fold (fun x acc => YS.cardinal (f x) + acc) xs 0.
+  Proof.
+    apply SetXS.set_induction with (s := xs); clear xs.
+    - intros xs Ex HD. rewrite flat_map_of_empty, SetXS.fold_1b; try assumption.
+      rewrite SetYS.cardinal_1; [reflexivity | apply YS.empty_spec].
+    - intros xs xxs IH x Nin Hadd HD. 
+End Set2.
+
+(* Theorem set_ind (P: set A -> Prop): *)
+(*   P empty -> *)
+(*   (forall (xs: set A) (x: A), P xs -> P (add x xs)) -> *)
+(*   forall xs: set A, P xs. *)
+(* Proof. *)
+(*   subst empty add union. *)
+(* Theorem union_empty_r (xs: set A): union xs empty = xs. *)
+(* Proof. reflexivity. Qed. *)
+
+(* Theorem union_empty_l (xs: set A): union empty xs = xs. *)
+(* Proof. *)
+(*   induction xs as [|x xs IH]; try reflexivity. *)
+(*   simpl. rewrite IH.  *)
+
+(* Theorem union_sym (xs ys: set A): union xs ys = union ys xs. *)
+(* Proof.  *)
+(*   generalize dependent xs. *)
+(*   induction ys as [|y ys IH]; intros xs. *)
+(*   - simpl. *)
+
+(* Theorem union_size (xs ys: set A): *)
+(*   set_size (set_union Aeq_dec xs ys) *)
+(*   = set_size xs + set_size ys - set_size (set_inter Aeq_dec xs ys). *)
+(* Proof. *)
+(*   generalize dependent ys. *)
+(*   induction xs as [|x xs IH]; intro ys. *)
+(*   - simpl. *)
+
+(*  app_length (* length_app *). *)
+
