tapl/coq/03_arith/Term.v
@@ -1,0 +1,12 @@
+(* AST definition of simple Arith language *)
+Inductive Term: Set :=
+| TTrue
+| TFalse
+| TZero
+| TSucc (t: Term)
+| TPred (t: Term)
+| TIsZero (t: Term)
+| TIf (cond thenBr elseBr: Term).
+
+Example TTrue_neq_TFalse: TTrue <> TFalse.
+Proof. discriminate. Qed.
